rhgfwpg

LeanGrow/F/EnvironmentManagement/Tests/Sample.lean
@@ -137,14 +137,16 @@ elab "runTest4" i:num n:name : command => do
       (do
         let res ← sampleForwAll iter proof
         let mut all := []
-        for ⟨k,n,g,c⟩ in res do
-          let ppc ← c.mapM ppExpr
-          let ppg ← ppExpr g
-          let out := (s!"Context:\nGoal: {ppg}\nKind : {repr k}\nName : {n}\n" : Format) ++ (Std.Format.join (ppc.map (fun y => y ++ ("\n" : Format))))
+        for ⟨k,n,g,c,ctx⟩ in res do
+          let out ← withLCtx ctx (← getLocalInstances) do
+            let ppc ← c.mapM ppExpr
+            let ppg ← ppExpr g
+            return (s!"Context:\nGoal: {ppg}\nKind : {repr k}\nName : {n}\n" : Format) ++ (Std.Format.join (ppc.map (fun y => y ++ ("\n" : Format))))
           all := out :: all
         return all
         : MetaM _)
   IO.println ((Std.Format.join (res.map (fun y => y ++ ("\n\n" : Format)))))
+
 
 
 
@@ -168,9 +170,8 @@ elab "runTest5" i:num n:name : command => do
   let .some proof := thm.value? | pure ()
   let iter := i.getNat
   let res ← Elab.Command.liftTermElabM
-    ((lambdaLetTelescope proof
-      (fun _ head => do
-        let res ← SampleForwAll iter head
+    (do
+        let res ← SampleForwAll iter proof
         let mut all := []
         for ⟨k,n,g,c⟩ in res do
           let ppc := c.map repr
@@ -178,8 +179,7 @@ elab "runTest5" i:num n:name : command => do
           let out := (s!"Context:\nGoal: {ppg}\nKind : {repr k}\nName : {n}\n" : Format) ++ (Std.Format.join (ppc.map (fun y => y ++ ("\n" : Format))))
           all := out :: all
         return all
-        )
-      (cleanupAnnotations := true)) : MetaM _)
+    : MetaM _)
   IO.println ((Std.Format.join (res.map (fun y => y ++ ("\n\n" : Format)))))
 
 
@@ -198,18 +198,17 @@ elab "runTest6" i:num n:name : command => do
   let .some proof := thm.value? | pure ()
   let iter := i.getNat
   let res ← Elab.Command.liftTermElabM
-    ((lambdaLetTelescope proof
-      (fun _ head => do
-        let res ← sampleBackAll iter head
-        let mut all := []
-        for ⟨k,n,g,c⟩ in res do
+    (do
+      let res ← sampleBackAll iter proof
+      let mut all := []
+      for ⟨k,n,g,c,ctx⟩ in res do
+        let out ← withLCtx ctx (← getLocalInstances) do
           let ppc ← c.mapM ppExpr
           let ppg ← ppExpr g
-          let out := (s!"Context:\nGoal: {ppg}\nKind : {repr k}\nName : {n}\n" : Format) ++ (Std.Format.join (ppc.map (fun y => y ++ ("\n" : Format))))
-          all := out :: all
-        return all
-        )
-      (cleanupAnnotations := true)) : MetaM _)
+          return (s!"Context:\nGoal: {ppg}\nKind : {repr k}\nName : {n}\n" : Format) ++ (Std.Format.join (ppc.map (fun y => y ++ ("\n" : Format))))
+        all := out :: all
+      return all
+      : MetaM _)
   IO.println ((Std.Format.join (res.map (fun y => y ++ ("\n\n" : Format)))))
 
 
@@ -219,3 +218,41 @@ runTest6 1 `test1
 runTest6 1 `test2
 runTest6 2 `test2
 runTest6 3 `test2
+
+
+theorem test3 : n + 0 = n := --by
+  Nat.recAux (Eq.refl (0 + 0)) (fun n _ ↦ Eq.refl (n + 1 + 0)) n
+  -- induction' n with n _
+  -- · rfl
+  -- · rfl
+
+runTest4 0 `test3
+runTest4 1 `test3
+runTest4 2 `test3
+
+runTest6 0 `test3
+runTest6 1 `test3
+runTest6 2 `test3
+
+def fac : Nat → Nat
+| 0 => 1
+| n+1 => n.succ * fac n
+
+theorem test4 (n : Nat) : fac n ≥ 1 := by
+  apply @Nat.rec (fun m => fac m ≥ 1)
+  -- induction' n with n ih
+  · apply Nat.le_refl
+  · intro n ih
+    apply Nat.le_trans ih
+    apply Nat.le_mul_of_pos_left
+    apply Nat.succ_pos
+
+#print test4
+
+runTest4 0 `test4
+runTest4 1 `test4
+runTest4 2 `test4
+
+runTest6 0 `test4
+runTest6 1 `test4
+runTest6 2 `test4
